Updates.

HandbookOfPracticalLogicLean/Chapter2/NF/DNF/PureDNF.lean
@@ -12,311 +12,106 @@ set_option autoImplicit false
 open Formula_
 
 
-def pure_dnf :
+/--
+  Helper function for `to_dnf_v3`.
+-/
+def to_dnf_v3_aux_1 :
   Formula_ → List (List Formula_)
-  | and_ p q => all_pairs_v4 List.union (pure_dnf p) (pure_dnf q)
-  | or_ p q => (pure_dnf p) ∪ (pure_dnf q)
+  | and_ p q => all_pairs_v4 List.union (to_dnf_v3_aux_1 p) (to_dnf_v3_aux_1 q)
+  | or_ p q => (to_dnf_v3_aux_1 p) ∪ (to_dnf_v3_aux_1 q)
   | F => [[F]]
 
-#eval (pure_dnf (Formula_| ((p \/ (q /\ r)) /\ (~p \/ ~ r)))).toString
+#eval (to_dnf_v3_aux_1 (Formula_| ((p \/ (q /\ r)) /\ (~p \/ ~ r)))).toString
 
 
-def dnf_list_of_list_to_formula
-  (l : List (List Formula_)) :
+/--
+  Helper function for `to_dnf_v3`.
+-/
+def to_dnf_v3_aux_2
+  (ll : List (List Formula_)) :
   Formula_ :=
-  list_disj (List.map list_conj l)
+  list_disj (List.map list_conj ll)
 
 
-#eval (dnf_list_of_list_to_formula [[atom_ "P", atom_ "Q"], [not_ (atom_ "P"), atom_ "R"]]).toString
-
-
-lemma dnf_list_of_list_to_formula_singleton
+/--
+  `to_dnf_v3 F` := Translates the formula `F` to a logically equivalent formula. If `F` is in negation normal form then `to_dnf_v3 F` is in disjunctive normal form.
+-/
+def to_dnf_v3
   (F : Formula_) :
-  dnf_list_of_list_to_formula [[F]] = F :=
-  by
-  unfold dnf_list_of_list_to_formula
-  simp only [List.map_cons, List.map_nil]
-  unfold list_conj
-  unfold list_disj
-  rfl
+  Formula_ :=
+  to_dnf_v3_aux_2 (to_dnf_v3_aux_1 F)
 
 
-lemma mem_list_mem_pure_dnf_of_nnf_v1_imp_is_constant_or_literal
-  (F : Formula_)
-  (l : List Formula_)
-  (P : Formula_)
-  (h1 : is_nnf_rec_v1 F)
-  (h2 : l ∈ pure_dnf F)
-  (h3 : P ∈ l) :
-  is_constant_ind P ∨ is_literal_ind P :=
-  by
-  induction F generalizing l
-  case false_ =>
-    unfold pure_dnf at h2
-    simp only [List.mem_singleton] at h2
-    rewrite [h2] at h3
-
-    simp only [List.mem_singleton] at h3
-    rewrite [h3]
-
-    left
-    apply is_constant_ind.rule_1
-  case true_ =>
-    unfold pure_dnf at h2
-    simp only [List.mem_singleton] at h2
-    rewrite [h2] at h3
-
-    simp only [List.mem_singleton] at h3
-    rewrite [h3]
-
-    left
-    apply is_constant_ind.rule_2
-  case atom_ X =>
-    unfold pure_dnf at h2
-    simp only [List.mem_singleton] at h2
-    rewrite [h2] at h3
-
-    simp only [List.mem_singleton] at h3
-    rewrite [h3]
-
-    right
-    apply is_literal_ind.rule_1
-  case not_ phi ih =>
-    unfold pure_dnf at h2
-    simp only [List.mem_singleton] at h2
-    rewrite [h2] at h3
-
-    simp only [List.mem_singleton] at h3
-    rewrite [h3]
-
-    cases phi
-    case atom_ X =>
-      right
-      apply is_literal_ind.rule_2
-    all_goals
-      unfold is_nnf_rec_v1 at h1
-      contradiction
-  case and_ phi psi phi_ih psi_ih =>
-    unfold is_nnf_rec_v1 at h1
-    obtain ⟨h1_left, h1_right⟩ := h1
-
-    unfold pure_dnf at h2
-
-    obtain s1 := mem_all_pairs_v4_union_imp_eq_union (pure_dnf phi) (pure_dnf psi) l h2
-    obtain ⟨xs, ys, xs_mem, ys_mem, eq⟩ := s1
-    rewrite [← eq] at h3
-
-    simp only [List.mem_union_iff] at h3
-    cases h3
-    case inl h3 =>
-      apply phi_ih xs
-      · exact h1_left
-      · exact xs_mem
-      · exact h3
-    case inr h3 =>
-      apply psi_ih ys
-      · exact h1_right
-      · exact ys_mem
-      · exact h3
-  case or_ phi psi phi_ih psi_ih =>
-    unfold is_nnf_rec_v1 at h1
-    obtain ⟨h1_left, h1_right⟩ := h1
-
-    unfold pure_dnf at h2
-    simp only [List.mem_union_iff] at h2
-
-    cases h2
-    case inl h2 =>
-      apply phi_ih l
-      · exact h1_left
-      · exact h2
-      · exact h3
-    case inr h2 =>
-      apply psi_ih l
-      · exact h1_right
-      · exact h2
-      · exact h3
-  all_goals
-    unfold is_nnf_rec_v1 at h1
-    contradiction
+#eval (to_dnf_v3_aux_2 [[atom_ "P", atom_ "Q"], [not_ (atom_ "P"), atom_ "R"]]).toString
 
 
-lemma is_nnf_v1_imp_pure_dnf_is_ind
-  (F : Formula_)
-  (h1 : is_nnf_rec_v1 F) :
-  is_dnf_ind_v1 (dnf_list_of_list_to_formula (pure_dnf F)) :=
-  by
-  cases F
-  case false_ =>
-    unfold pure_dnf
-    simp only [dnf_list_of_list_to_formula_singleton]
-    apply is_dnf_ind_v1.rule_1
-    apply is_conj_ind_v1.rule_1
-    apply is_constant_ind.rule_1
-  case true_ =>
-    unfold pure_dnf
-    simp only [dnf_list_of_list_to_formula_singleton]
-    apply is_dnf_ind_v1.rule_1
-    apply is_conj_ind_v1.rule_1
-    apply is_constant_ind.rule_2
-  case atom_ X =>
-    unfold pure_dnf
-    simp only [dnf_list_of_list_to_formula_singleton]
-    apply is_dnf_ind_v1.rule_1
-    apply is_conj_ind_v1.rule_2
-    apply is_literal_ind.rule_1
-  case not_ phi =>
-    unfold pure_dnf
-    simp only [dnf_list_of_list_to_formula_singleton]
-    cases phi
-    case atom_ X =>
-      apply is_dnf_ind_v1.rule_1
-      apply is_conj_ind_v1.rule_2
-      apply is_literal_ind.rule_2
-    all_goals
-      unfold is_nnf_rec_v1 at h1
-      contradiction
-  case and_ phi psi =>
-    unfold is_nnf_rec_v1 at h1
-    obtain ⟨h1_left, h1_right⟩ := h1
-
-    unfold pure_dnf
-    unfold dnf_list_of_list_to_formula
-    apply list_disj_of_is_conj_ind_v1_is_dnf_ind_v1
-    intro F a1
-    simp only [List.mem_map] at a1
-    obtain ⟨l, a1_left, a1_right⟩ := a1
-    rewrite [← a1_right]
-    apply list_conj_of_list_of_is_constant_ind_or_is_literal_ind_is_conj_ind_v1
-    intro P a2
-
-    obtain s1 := mem_all_pairs_v4_union_imp_eq_union (pure_dnf phi) (pure_dnf psi) l a1_left
-    obtain ⟨xs, ys, xs_mem, ys_mem, eq⟩ := s1
-    rewrite [← eq] at a2
-    simp only [List.mem_union_iff] at a2
-
-    cases a2
-    case inl a2 =>
-      apply mem_list_mem_pure_dnf_of_nnf_v1_imp_is_constant_or_literal phi xs
-      · exact h1_left
-      · exact xs_mem
-      · exact a2
-    case inr a2 =>
-      apply mem_list_mem_pure_dnf_of_nnf_v1_imp_is_constant_or_literal psi ys
-      · exact h1_right
-      · exact ys_mem
-      · exact a2
-  case or_ phi psi =>
-    unfold is_nnf_rec_v1 at h1
-    obtain ⟨h1_left, h1_right⟩ := h1
-
-    unfold pure_dnf
-    unfold dnf_list_of_list_to_formula
-    apply list_disj_of_is_conj_ind_v1_is_dnf_ind_v1
-    intro F a1
-    simp only [List.mem_map, List.mem_union_iff] at a1
-    obtain ⟨l, a1_left, a1_right⟩ := a1
-    rewrite [← a1_right]
-    apply list_conj_of_list_of_is_constant_ind_or_is_literal_ind_is_conj_ind_v1
-    intro P a2
-
-    cases a1_left
-    case inl a1_left =>
-      apply mem_list_mem_pure_dnf_of_nnf_v1_imp_is_constant_or_literal phi l
-      · exact h1_left
-      · exact a1_left
-      · exact a2
-    case inr a1_left =>
-      apply mem_list_mem_pure_dnf_of_nnf_v1_imp_is_constant_or_literal psi l
-      · exact h1_right
-      · exact a1_left
-      · exact a2
-  all_goals
-    unfold is_nnf_rec_v1 at h1
-    contradiction
-
-
-lemma eval_dnf_list_of_list_to_formula_pure_dnf_eq_eval
+example
   (V : ValuationAsTotalFunction)
   (F : Formula_) :
-  eval V (dnf_list_of_list_to_formula (pure_dnf F)) = true ↔ eval V F = true :=
+  eval V F = true ↔ eval V (to_dnf_v3 F) = true :=
   by
+  unfold to_dnf_v3
   induction F
   case and_ phi psi phi_ih psi_ih =>
-    unfold dnf_list_of_list_to_formula at phi_ih
-    unfold dnf_list_of_list_to_formula at psi_ih
+    unfold to_dnf_v3_aux_2 at phi_ih
 
-    unfold pure_dnf
-    unfold dnf_list_of_list_to_formula
+    unfold to_dnf_v3_aux_2 at psi_ih
+
+    unfold to_dnf_v3_aux_1
+    unfold to_dnf_v3_aux_2
     simp only [eval]
     simp only [bool_iff_prop_and]
-    rewrite [← phi_ih]
-    rewrite [← psi_ih]
+    rewrite [phi_ih]
+    rewrite [psi_ih]
     simp only [eval_list_disj_eq_true_iff_exists_eval_eq_true]
     simp only [List.mem_map]
     simp only [mem_all_pairs_v4_union_iff_eq_union]
     constructor
     · intro a1
-      obtain ⟨F, ⟨P, ⟨xs, ys, ⟨xs_mem, ys_mem, eq⟩⟩, a1_left⟩, a1_right⟩ := a1
+      obtain ⟨⟨p, ⟨l1, l1_mem, a1_left_left⟩, a1_left_right⟩ , ⟨Q, ⟨l2, l2_mem, a1_right_left⟩, a1_right_right⟩ ⟩ := a1
+      rewrite [← a1_left_left] at a1_left_right
+      rewrite [← a1_right_left] at a1_right_right
+      apply Exists.intro (list_conj (l1 ∪ l2))
+      constructor
+      · apply Exists.intro (l1 ∪ l2)
+        constructor
+        · apply Exists.intro l1
+          apply Exists.intro l2
+          exact ⟨l1_mem, l2_mem, rfl⟩
+        · rfl
+      · simp only [eval_list_conj_union]
+        exact ⟨a1_left_right, a1_right_right⟩
+    · intro a1
+      obtain ⟨F, ⟨p, ⟨l1, l2, ⟨l1_mem, l2_mem, eq⟩⟩, a1_left⟩, a1_right⟩ := a1
       rewrite [← a1_left] at a1_right
       rewrite [← eq] at a1_right
       simp only [eval_list_conj_union] at a1_right
       obtain ⟨a1_right_left, a1_right_right⟩ := a1_right
       constructor
-      · apply Exists.intro (list_conj xs)
+      · apply Exists.intro (list_conj l1)
         constructor
-        · apply Exists.intro xs
-          exact ⟨xs_mem, rfl⟩
+        · apply Exists.intro l1
+          exact ⟨l1_mem, rfl⟩
         · exact a1_right_left
-      · apply Exists.intro (list_conj ys)
+      · apply Exists.intro (list_conj l2)
         constructor
-        · apply Exists.intro ys
-          exact ⟨ys_mem, rfl⟩
+        · apply Exists.intro l2
+          exact ⟨l2_mem, rfl⟩
         · exact a1_right_right
-    · intro a1
-      obtain ⟨⟨P, ⟨xs, xs_mem, a1_left_left⟩, a1_left_right⟩ , ⟨Q, ⟨ys, ys_mem, a1_right_left⟩, a1_right_right⟩ ⟩ := a1
-      rewrite [← a1_left_left] at a1_left_right
-      rewrite [← a1_right_left] at a1_right_right
-      apply Exists.intro (list_conj (xs ∪ ys))
-      constructor
-      · apply Exists.intro (xs ∪ ys)
-        constructor
-        · apply Exists.intro xs
-          apply Exists.intro ys
-          exact ⟨xs_mem, ys_mem, rfl⟩
-        · rfl
-      · simp only [eval_list_conj_union]
-        exact ⟨a1_left_right, a1_right_right⟩
   case or_ phi psi phi_ih psi_ih =>
-    unfold dnf_list_of_list_to_formula at phi_ih
-    unfold dnf_list_of_list_to_formula at psi_ih
+    unfold to_dnf_v3_aux_2 at phi_ih
 
-    unfold pure_dnf
-    unfold dnf_list_of_list_to_formula
+    unfold to_dnf_v3_aux_2 at psi_ih
+
+    unfold to_dnf_v3_aux_1
+    unfold to_dnf_v3_aux_2
     simp only [eval]
     simp only [bool_iff_prop_or]
-    rewrite [← phi_ih]
-    rewrite [← psi_ih]
+    rewrite [phi_ih]
+    rewrite [psi_ih]
     simp only [eval_list_disj_eq_true_iff_exists_eval_eq_true]
     simp only [List.mem_map, List.mem_union_iff]
     constructor
-    · intro a1
-      obtain ⟨F, ⟨l, a1_left_left, a1_left_right⟩, a1_right⟩ := a1
-      cases a1_left_left
-      case inl a1_left_left =>
-        left
-        apply Exists.intro F
-        constructor
-        · apply Exists.intro l
-          exact ⟨a1_left_left, a1_left_right⟩
-        · exact a1_right
-      case inr a1_left_left =>
-        right
-        apply Exists.intro F
-        constructor
-        · apply Exists.intro l
-          exact ⟨a1_left_left, a1_left_right⟩
-        · exact a1_right
     · intro a1
       cases a1
       case inl a1 =>
@@ -339,5 +134,238 @@ lemma eval_dnf_list_of_list_to_formula_pure_dnf_eq_eval
             exact a1_left_left
           · exact a1_left_right
         · exact a1_right
+    · intro a1
+      obtain ⟨F, ⟨l, a1_left_left, a1_left_right⟩, a1_right⟩ := a1
+      cases a1_left_left
+      case inl a1_left_left =>
+        left
+        apply Exists.intro F
+        constructor
+        · apply Exists.intro l
+          exact ⟨a1_left_left, a1_left_right⟩
+        · exact a1_right
+      case inr a1_left_left =>
+        right
+        apply Exists.intro F
+        constructor
+        · apply Exists.intro l
+          exact ⟨a1_left_left, a1_left_right⟩
+        · exact a1_right
   all_goals
     rfl
+
+
+-------------------------------------------------------------------------------
+
+
+lemma to_dnf_v3_aux_2_singleton
+  (F : Formula_) :
+  to_dnf_v3_aux_2 [[F]] = F :=
+  by
+  unfold to_dnf_v3_aux_2
+  simp only [List.map_cons, List.map_nil]
+  unfold list_conj
+  unfold list_disj
+  rfl
+
+
+lemma mem_list_mem_to_dnf_v3_aux_1_of_nnf_rec_v1_imp_is_constant_or_literal
+  (F : Formula_)
+  (l : List Formula_)
+  (p : Formula_)
+  (h1 : is_nnf_rec_v1 F)
+  (h2 : l ∈ to_dnf_v3_aux_1 F)
+  (h3 : p ∈ l) :
+  is_constant_ind p ∨ is_literal_ind p :=
+  by
+  induction F generalizing l
+  case false_ =>
+    unfold to_dnf_v3_aux_1 at h2
+    simp only [List.mem_singleton] at h2
+    rewrite [h2] at h3
+
+    simp only [List.mem_singleton] at h3
+    rewrite [h3]
+
+    left
+    apply is_constant_ind.rule_1
+  case true_ =>
+    unfold to_dnf_v3_aux_1 at h2
+    simp only [List.mem_singleton] at h2
+    rewrite [h2] at h3
+
+    simp only [List.mem_singleton] at h3
+    rewrite [h3]
+
+    left
+    apply is_constant_ind.rule_2
+  case atom_ X =>
+    unfold to_dnf_v3_aux_1 at h2
+    simp only [List.mem_singleton] at h2
+    rewrite [h2] at h3
+
+    simp only [List.mem_singleton] at h3
+    rewrite [h3]
+
+    right
+    apply is_literal_ind.rule_1
+  case not_ phi ih =>
+    unfold to_dnf_v3_aux_1 at h2
+    simp only [List.mem_singleton] at h2
+    rewrite [h2] at h3
+
+    simp only [List.mem_singleton] at h3
+    rewrite [h3]
+
+    cases phi
+    case atom_ X =>
+      right
+      apply is_literal_ind.rule_2
+    all_goals
+      unfold is_nnf_rec_v1 at h1
+      contradiction
+  case and_ phi psi phi_ih psi_ih =>
+    unfold is_nnf_rec_v1 at h1
+    obtain ⟨h1_left, h1_right⟩ := h1
+
+    unfold to_dnf_v3_aux_1 at h2
+
+    obtain s1 := mem_all_pairs_v4_union_imp_eq_union (to_dnf_v3_aux_1 phi) (to_dnf_v3_aux_1 psi) l h2
+    obtain ⟨l1, l2, l1_mem, l2_mem, eq⟩ := s1
+
+    rewrite [← eq] at h3
+    simp only [List.mem_union_iff] at h3
+
+    cases h3
+    case inl h3 =>
+      apply phi_ih l1
+      · exact h1_left
+      · exact l1_mem
+      · exact h3
+    case inr h3 =>
+      apply psi_ih l2
+      · exact h1_right
+      · exact l2_mem
+      · exact h3
+  case or_ phi psi phi_ih psi_ih =>
+    unfold is_nnf_rec_v1 at h1
+    obtain ⟨h1_left, h1_right⟩ := h1
+
+    unfold to_dnf_v3_aux_1 at h2
+    simp only [List.mem_union_iff] at h2
+
+    cases h2
+    case inl h2 =>
+      apply phi_ih l
+      · exact h1_left
+      · exact h2
+      · exact h3
+    case inr h2 =>
+      apply psi_ih l
+      · exact h1_right
+      · exact h2
+      · exact h3
+  all_goals
+    unfold is_nnf_rec_v1 at h1
+    contradiction
+
+
+lemma is_nnf_rec_v1_imp_to_dnf_v3_is_dnf_ind_v1
+  (F : Formula_)
+  (h1 : is_nnf_rec_v1 F) :
+  is_dnf_ind_v1 (to_dnf_v3 F) :=
+  by
+  cases F
+  case false_ =>
+    unfold to_dnf_v3
+    unfold to_dnf_v3_aux_1
+    simp only [to_dnf_v3_aux_2_singleton]
+    apply is_dnf_ind_v1.rule_1
+    apply is_conj_ind_v1.rule_1
+    apply is_constant_ind.rule_1
+  case true_ =>
+    unfold to_dnf_v3
+    unfold to_dnf_v3_aux_1
+    simp only [to_dnf_v3_aux_2_singleton]
+    apply is_dnf_ind_v1.rule_1
+    apply is_conj_ind_v1.rule_1
+    apply is_constant_ind.rule_2
+  case atom_ X =>
+    unfold to_dnf_v3
+    unfold to_dnf_v3_aux_1
+    simp only [to_dnf_v3_aux_2_singleton]
+    apply is_dnf_ind_v1.rule_1
+    apply is_conj_ind_v1.rule_2
+    apply is_literal_ind.rule_1
+  case not_ phi =>
+    unfold to_dnf_v3
+    unfold to_dnf_v3_aux_1
+    simp only [to_dnf_v3_aux_2_singleton]
+    cases phi
+    case atom_ X =>
+      apply is_dnf_ind_v1.rule_1
+      apply is_conj_ind_v1.rule_2
+      apply is_literal_ind.rule_2
+    all_goals
+      unfold is_nnf_rec_v1 at h1
+      contradiction
+  case and_ phi psi =>
+    unfold is_nnf_rec_v1 at h1
+    obtain ⟨h1_left, h1_right⟩ := h1
+
+    apply list_disj_of_is_conj_ind_v1_is_dnf_ind_v1
+    intro F a1
+    simp only [List.mem_map] at a1
+    obtain ⟨l, a1_left, a1_right⟩ := a1
+    rewrite [← a1_right]
+    apply list_conj_of_list_of_is_constant_ind_or_is_literal_ind_is_conj_ind_v1
+    intro P a2
+
+    obtain s1 := mem_all_pairs_v4_union_imp_eq_union (to_dnf_v3_aux_1 phi) (to_dnf_v3_aux_1 psi) l a1_left
+    obtain ⟨l1, l2, l1_mem, l2_mem, eq⟩ := s1
+    rewrite [← eq] at a2
+    simp only [List.mem_union_iff] at a2
+
+    cases a2
+    case inl a2 =>
+      apply mem_list_mem_to_dnf_v3_aux_1_of_nnf_rec_v1_imp_is_constant_or_literal phi l1
+      · exact h1_left
+      · exact l1_mem
+      · exact a2
+    case inr a2 =>
+      apply mem_list_mem_to_dnf_v3_aux_1_of_nnf_rec_v1_imp_is_constant_or_literal psi l2
+      · exact h1_right
+      · exact l2_mem
+      · exact a2
+  case or_ phi psi =>
+    unfold is_nnf_rec_v1 at h1
+    obtain ⟨h1_left, h1_right⟩ := h1
+
+    unfold to_dnf_v3
+    unfold to_dnf_v3_aux_1
+    unfold to_dnf_v3_aux_2
+    apply list_disj_of_is_conj_ind_v1_is_dnf_ind_v1
+    intro F a1
+    simp only [List.mem_map, List.mem_union_iff] at a1
+    obtain ⟨l, a1_left, a1_right⟩ := a1
+    rewrite [← a1_right]
+    apply list_conj_of_list_of_is_constant_ind_or_is_literal_ind_is_conj_ind_v1
+    intro P a2
+
+    cases a1_left
+    case inl a1_left =>
+      apply mem_list_mem_to_dnf_v3_aux_1_of_nnf_rec_v1_imp_is_constant_or_literal phi l
+      · exact h1_left
+      · exact a1_left
+      · exact a2
+    case inr a1_left =>
+      apply mem_list_mem_to_dnf_v3_aux_1_of_nnf_rec_v1_imp_is_constant_or_literal psi l
+      · exact h1_right
+      · exact a1_left
+      · exact a2
+  all_goals
+    unfold is_nnf_rec_v1 at h1
+    contradiction
+
+
+#lint
